Semantic/CC/Eval/BigStep.lean
@@ -13,11 +13,11 @@ inductive Eval : Heap -> Exp {} -> Hpost -> Prop where
   (hQ : Q (.var x) h) ->
   Eval h (.var x) Q
 | eval_apply {h : Heap} {x : Nat} :
-  h x = some ⟨.abs T e, hv⟩ ->
+  h x = some (.val ⟨.abs T e, hv⟩) ->
   Eval h (e.subst (Subst.openVar y)) Q ->
   Eval h (.app (.free x) y) Q
 | eval_tapply {h : Heap} {x : Nat} :
-  h x = some ⟨.tabs T0 e, hv⟩ ->
+  h x = some (.val ⟨.tabs T0 e, hv⟩) ->
   Eval h (e.subst (Subst.openTVar .top)) Q ->
   Eval h (.tapp (.free x) S) Q
 | eval_letin {h : Heap} {Q1 : Hpost} :
